changed funcs_ok so that Stub.v can go through. Need to fix statement compiler

platform/cito/GoodFunction.v
@@ -1,45 +1,35 @@
 Set Implicit Arguments.
 
 Require Import GoodFunc.
+Require Import SyntaxFunc.
+Export SyntaxFunc.
 
 Record GoodFunction := 
   {
-    Name : string;
-    ArgVars : list string;
-    RetVar : string;
-    Body : Stmt;
-    NoDupArgVars : NoDup ArgVars;
-    WellFormedBody : WellFormed Body
+    Fun : Func;
+    NoDupArgVars : NoDup (ArgVars Fun);
+    WellFormedBody : WellFormed (Body Fun)
   }.
+
+Coercion Fun : GoodFunction >-> Func.
     
-Definition to_good_function f : GoodFunc f -> GoodFunction.
+Definition to_good_function (f : Func) : GoodFunc f -> GoodFunction.
     intros.
     destruct H.
     econstructor.
-    eapply (SyntaxFunc.Name f).
-    eapply (SyntaxFunc.RetVar f).
     eauto.
     eauto.
 Defined.
 
-Lemma to_good_function_name : forall f (H : GoodFunc.GoodFunc f), Name (to_good_function H) = SyntaxFunc.Name f.
+Lemma to_good_function_name : forall (f : Func) (H : GoodFunc f), Name (to_good_function f H) = SyntaxFunc.Name f.
   intros.
   destruct H.
   unfold to_good_function.
   eauto.
 Qed.
 
-Definition to_func (f : GoodFunction) : SyntaxFunc.Func :=
-  {|
-    SyntaxFunc.Name := Name f;
-    SyntaxFunc.ArgVars := ArgVars f;
-    SyntaxFunc.RetVar := RetVar f;
-    SyntaxFunc.Body := Body f
-  |}.
-
-Lemma to_func_good : forall f, GoodFunc (to_func f).
+Lemma to_func_good : forall (f : GoodFunction), GoodFunc f.
   intros.
-  unfold to_func.
   destruct f.
   split; simpl; eauto.
 Qed.    
