platform/cito/GoodModule.v
@@ -1,9 +1,10 @@
 Set Implicit Arguments.
 
 Require Import GoodFunction.
+
 Record GoodModule :=
   {
     Name : string;
     Functions : list GoodFunction;
-    NoDupFuncNames : NoDup (map GoodFunction.Name Functions)
+    NoDupFuncNames : NoDup (map (fun (f : GoodFunction) => SyntaxFunc.Name f) Functions)
   }.
