platform/cito/Inv.v
@@ -12,17 +12,17 @@ Definition empty_vs : vals := fun _ => $0.
 
 Section TopSection.
 
-  Definition has_extra_stack sp offset e_stack :=
+  Definition has_extra_stack sp offset e_stack e_stack_real :=
     ((sp ^+ $4) =*> $(e_stack) *
-     (sp ^+ $8 ^+ $(4 * offset)) =?> e_stack)%Sep.
+     (sp ^+ $8 ^+ $(4 * offset)) =?> e_stack_real)%Sep.
 
-  Definition is_state sp rp e_stack vars (v : State) temps : HProp :=
+  Definition is_state sp rp e_stack e_stack_real vars (v : State) temps : HProp :=
     (
      locals vars (fst v) 0 (sp ^+ $8) *
      array temps (sp ^+ $8 ^+ $(4 * length vars)) *
      is_heap (snd v) *
      sp =*> rp *
-     has_extra_stack sp (length vars + length temps) e_stack
+     has_extra_stack sp (length vars + length temps) e_stack e_stack_real
     )%Sep.
 
   Require Import Malloc.
@@ -49,44 +49,63 @@ Section TopSection.
 
   Fixpoint make_heap pairs := fold_left store_pair pairs heap_empty.
 
-  Definition funcs_ok (stn : settings) (fs : W -> option Callee) : PropX W (settings * state) := 
-    let env := (Labels stn, fs) in
-    ((Al i, Al spec, 
-      [| fs i = Some (Internal spec) |] 
-        ---> (i, stn) @@@ (
-          st ~> ExX, Ex v, Ex rp, Ex e_stack,
-          ![^[is_state st#Sp rp e_stack (ArgVars spec) v nil * mallocHeap 0] * #0] st /\
-          [| Safe env (Body spec) v |] /\
-          (st#Rp, stn) 
-            @@@ (
-              st' ~> Ex v', Ex rp',
-              ![^[ is_state st'#Sp rp' e_stack (ArgVars spec) v' nil * mallocHeap 0] * #1] st' /\
-              [| exists vs', 
-                 RunsTo env (Body spec) v (vs', snd v') /\ 
-                 st'#Rv = sel vs' (RetVar spec) /\
-                 st'#Sp = st#Sp |]))) /\
-     (Al i, Al spec, 
-      [| fs i = Some (Foreign spec) |] 
-        ---> (i, stn) @@@ (
-          st ~> ExX, Ex pairs, Ex rp, Ex e_stack,
-          let heap := make_heap pairs in
-          ![^[is_state st#Sp rp e_stack nil (empty_vs, heap) (map fst pairs) * mallocHeap 0] * #0] st /\
-          [| disjoint_ptrs pairs /\
-             PreCond spec (map snd pairs) |] /\
-          (st#Rp, stn) 
-            @@@ (
-              st' ~> Ex args', Ex addr, Ex ret, Ex rp', Ex outs,
-              let t := decide_ret addr ret in
-              let ret_w := fst t in
-              let ret_a := snd t in
-              let triples := make_triples pairs outs in
-              let heap := fold_left store_out triples heap in
-              ![^[is_state st#Sp rp' e_stack nil (empty_vs, heap) args' * layout_option ret_w ret_a * mallocHeap 0] * #1] st' /\
-              [| length outs = length pairs /\
-                 PostCond spec (map (fun x => (ADTIn x, ADTOut x)) triples) ret /\
-                 length args' = length triples /\
-                 st'#Rv = ret_w /\
-                 st'#Sp = st#Sp |]))))%PropX.
+  Open Scope type.
+
+  Require Import ConvertLabel.
+  Definition internal_spec G fs spec st : propX _ _ (settings * smem :: G) :=
+    (Ex v, Ex rp, Ex e_stack,
+     ![^[is_state st#Sp rp e_stack e_stack (ArgVars spec) v nil * mallocHeap 0] * #0] st /\
+     let stn := fst st in
+     let env := (from_bedrock_label_map (Labels stn), fs stn) in
+     [| Safe env (Body spec) v |] /\
+     (st#Rp, stn) 
+       @@@ (
+         st' ~> Ex v', Ex rp', 
+         (* the callee needn't have the right extra stack size recorded in the end, but the extra stack should be there *)
+         Ex e_stack',
+         ![^[ is_state st'#Sp rp' e_stack' e_stack (ArgVars spec) v' nil * mallocHeap 0] * #1] st' /\
+         [| exists vs', 
+            RunsTo env (Body spec) v (vs', snd v') /\ 
+            st'#Rv = sel vs' (RetVar spec) /\
+            st'#Sp = st#Sp |]))%PropX.
+
+  Definition foreign_spec G spec st : propX _ _ (settings * smem :: G) :=
+    (Ex pairs, Ex rp, Ex e_stack,
+     let heap := make_heap pairs in
+     ![^[is_state st#Sp rp e_stack e_stack nil (empty_vs, heap) (map fst pairs) * mallocHeap 0] * #0] st /\
+     let stn := fst st in
+     [| disjoint_ptrs pairs /\
+        PreCond spec (map snd pairs) |] /\
+     (st#Rp, stn) 
+       @@@ (
+         st' ~> Ex args', Ex addr, Ex ret, Ex rp', Ex outs,
+         let t := decide_ret addr ret in
+         let ret_w := fst t in
+         let ret_a := snd t in
+         let triples := make_triples pairs outs in
+         let heap := fold_left store_out triples heap in
+         (* the callee needn't have the right extra stack size recorded in the end, but the extra stack should be there *)
+         Ex e_stack',
+         ![^[is_state st#Sp rp' e_stack' e_stack nil (empty_vs, heap) args' * layout_option ret_w ret_a * mallocHeap 0] * #1] st' /\
+         [| length outs = length pairs /\
+            PostCond spec (map (fun x => (ADTIn x, ADTOut x)) triples) ret /\
+            length args' = length triples /\
+            st'#Rv = ret_w /\
+            st'#Sp = st#Sp |]))%PropX.
+
+  Definition cptr_AlX G (p : W) (stn : settings) a : propX _ _ G :=
+    (ExX, 
+     Cptr p #0 /\
+     Al st : state, AlX : settings * smem,
+     a (stn, st) ---> #1 (stn, st))%PropX.
+    
+  Definition funcs_ok (fs : settings -> W -> option Callee) : PropX W (settings * state) := 
+    ((Al i, Al stn, Al spec,
+      [| fs stn i = Some (Internal spec) |] 
+        ---> cptr_AlX i stn (internal_spec _ fs spec)) /\
+     (Al i, Al stn, Al spec, 
+      [| fs stn i = Some (Foreign spec) |] 
+        ---> cptr_AlX i stn (foreign_spec _ spec)))%PropX.
 
   Section vars.
 
@@ -96,18 +115,18 @@ Section TopSection.
 
     Definition inv_template rv_precond rv_postcond s : assert := 
       st ~> Ex fs, 
-      let stn := fst st in
-      let env := (Labels stn, fs) in
-      funcs_ok stn fs /\
+      funcs_ok fs /\
       ExX, Ex v, Ex temps, Ex rp, Ex e_stack,
-      ![^[is_state st#Sp rp e_stack vars v temps * mallocHeap 0] * #0] st /\
+      ![^[is_state st#Sp rp e_stack e_stack vars v temps * mallocHeap 0] * #0] st /\
+      let stn := fst st in
+      let env := (from_bedrock_label_map (Labels stn), fs stn) in
       [| Safe env s v /\
          length temps = temp_size /\
          rv_precond st#Rv v |] /\
       (rp, stn) 
         @@@ (
           st' ~> Ex v', Ex temps',
-          ![^[is_state st'#Sp rp e_stack vars v' temps' * mallocHeap 0] * #1] st' /\
+          ![^[is_state st'#Sp rp e_stack e_stack vars v' temps' * mallocHeap 0] * #1] st' /\
           [| RunsTo env s v v' /\
              length temps' = temp_size /\
              st'#Sp = st#Sp /\
